thys/Group-Ring-Module/Algebra5.thy
@@ -1465,7 +1465,7 @@ done
 
 lemma (in Ring) prime_ideal_cont1Tr:"ideal R A  \<Longrightarrow> 
       \<forall>P. ((P \<in> {j. j \<le> (n::nat)} \<rightarrow> {X. prime_ideal R X}) \<and> 
-                   (A \<subseteq> \<Union> P ` {j. j \<le> n})) \<longrightarrow> (\<exists>i\<le> n. A \<subseteq> (P i))"
+                   (A \<subseteq> \<Union> (P ` {j. j \<le> n}))) \<longrightarrow> (\<exists>i\<le> n. A \<subseteq> (P i))"
 apply (induct_tac n)
  apply (rule allI, rule impI)
  apply (erule conjE)
@@ -1484,7 +1484,7 @@ apply (rule allI, rule impI)
                simp+, erule conjE, simp add:compose_def,blast)
  (** last_step induction assumption is of no use **)
 apply (thin_tac "\<forall>P. P \<in> {j. j \<le> n} \<rightarrow> {X. prime_ideal R X} \<and>
-               A \<subseteq> \<Union>P ` {j. j \<le> n} \<longrightarrow>
+               A \<subseteq> \<Union>(P ` {j. j \<le> n}) \<longrightarrow>
                (\<exists>i\<le>n. A \<subseteq> P i)",
        rule contrapos_pp, simp+)
  apply (cut_tac n = n and P = P in prod_prime [of A], assumption)
@@ -1531,7 +1531,7 @@ lemma (in Ring) prime_ideal_cont1:"\<lbrakk>ideal R A; \<forall>i \<le> (n::nat)
 apply (frule prime_ideal_cont1Tr[of A n])
 apply (frule_tac a = P in forall_spec,
        thin_tac "\<forall>P. P \<in> {j. j \<le> n} \<rightarrow> {X. prime_ideal R X} \<and> 
-       A \<subseteq> \<Union>P ` {j. j \<le> n} \<longrightarrow> (\<exists>i\<le>n. A \<subseteq> P i)")
+       A \<subseteq> \<Union>(P ` {j. j \<le> n}) \<longrightarrow> (\<exists>i\<le>n. A \<subseteq> P i)")
 apply (rule conjI, simp,
        rule subsetI, simp,
        frule_tac c = x in subsetD[of A "\<Union>{X. \<exists>i\<le>n. X = P i}"], assumption+,
