thys/Program-Conflict-Analysis/Semantics.thy
@@ -53,11 +53,11 @@ lemma mon_e_simps [simp]:
 definition
   "mon_w fg w == \<Union> { mon_e fg e | e. e \<in> set w}"
 
-lemma mon_s_alt: "mon_s fg s == \<Union> mon fg ` proc_of fg ` set s"
+lemma mon_s_alt: "mon_s fg s == \<Union> (mon fg ` proc_of fg ` set s)"
   by (unfold mon_s_def mon_n_def) (auto intro!: eq_reflection)
-lemma mon_c_alt: "mon_c fg c == \<Union> mon_s fg ` set_of c"
+lemma mon_c_alt: "mon_c fg c == \<Union> (mon_s fg ` set_of c)"
   by (unfold mon_c_def set_of_def) (auto intro!: eq_reflection)
-lemma mon_w_alt: "mon_w fg w == \<Union> mon_e fg ` set w"
+lemma mon_w_alt: "mon_w fg w == \<Union> (mon_e fg ` set w)"
   by (unfold mon_w_def) (auto intro!: eq_reflection)
 
 lemma mon_sI: "\<lbrakk>n\<in>set s; m\<in>mon_n fg n\<rbrakk> \<Longrightarrow> m\<in>mon_s fg s"
